

Binh Le SID

Hugo Wan SID

CS 111 ASSIGNMENT 3

Problem 1: a) Consider the following linear homogeneous recurrence relation: $R_n = 4R_{n-1} - 3R_{n-2}$. It is known that: $R_0 = 1$, $R_2 = 5$. Find R_3 .

Solution:

If $n = 2$, then $R_2 = 4R_{2-1} - 3R_{2-2} \implies R_2 = 4R_1 - 3R_0$

$\implies 5 = 4R_1 - 3 * 1 \implies 5 = 4R_1 - 3 \implies 8 = 4R_1 \implies R_1 = 2$

To find R_3 , $n = 3$, then $R_3 = 4R_{3-1} - 3R_{3-2} \implies R_3 = 4R_2 - 3R_1$

$\implies R_3 = 4 * 5 - 3 * 2 \implies R_3 = 20 - 6 \implies R_3 = 14$

Answer: $R_3 = 14$.

b) Determine the general solution of the recurrence equation if its characteristic equation has the following roots: 1, -2, -2, 2, 7, 7.

Solution:

The general solution of the recurrence equation:

$$R_n = a_1 * (1)^n + a_2 * (-2)^n + a_3 * n(-2)^n + a_4 * (2)^n + a_5 * (7)^n + a_6 * n(7)^n$$

c) Determine the general solution of the recurrence equation $A_n = 256A_{n-4}$.

Solution:

Characteristic equation is $x^4 = 256$. Its roots are 4 and -4.

General form of the solution: $A_n = a_1 * 4^n + a_2 * (-4)^n$

d) Find the general form of the particular solution of the recurrence $B_n = 3B_{n-2} - 2B_{n-3} + 2$.

Solution:

Characteristic equation and its roots: $x^3 - 3x - 2 = 0$, $x_1 = 1$, $x_2 = 1$, $x_3 = -2$

General solution of the homogeneous equation: $f'_n = a_1(1)^n + a_2n(1)^n + a_3(-2)^n$

Particular solution of the non-homogeneous equation: $f''_n = B$.

(Answer) The general form of the particular solution of the recurrence: $B = 3B(n-2) - 2B(n-3) + 2$

Plug in: $\implies n = 3, B = 3B - 0 + 2 \implies 2B = -2 \implies B = -1$

The general solution: $B_n = a_1(1)^n + a_2n(1)^n + a_3(-2)^n - 1$

Problem 2: Solve the following recurrence equations:

a)

$$f_n = f_{n-1} + 4f_{n-2} + 2f_{n-3}$$

$$f_0 = 0$$

$$f_1 = 1$$

$$f_2 = 4$$

Show your work (all steps: the characteristic polynomial and its roots, the general solution, using the initial conditions to compute the final solution.)

Solution:

The first step is to find the characteristic polynomial, which is $x^3 - x^2 - 4x - 2 = 0$, and from that, we can factor it into $(x+1)(x^2 - 2x - 2)$. One of the roots we get is -1 . Then we use the quadratic formula to find

the roots of $x^2 - 2x - 2$, and we get $1 + \sqrt{3}, 1 - \sqrt{3}$. So in sum,

Characteristic polynomial and its roots: $x^3 - x^2 - 4x - 2 = 0, x = -1, 1 + \sqrt{3}, 1 - \sqrt{3}$

General solution: $f_n = a_1(-1)^n + a_2(1 + \sqrt{3})^n + a_3(1 - \sqrt{3})^n$

Using the initial conditions:

$$f_0 = 0 = a_1(-1)^0 + a_2(1 + \sqrt{3})^0 + a_3(1 - \sqrt{3})^0 = a_1 + a_2 + a_3 \implies a_1 + a_2 + a_3 = 0$$

$$f_1 = 1 = a_1(-1)^1 + a_2(1 + \sqrt{3})^1 + a_3(1 - \sqrt{3})^1 \implies -a_1 + a_2(1 + \sqrt{3}) + a_3(1 - \sqrt{3}) = 1$$

$$\implies -a_1 + a_2 + \sqrt{3}a_2 + a_3 - \sqrt{3}a_3 = 1$$

$$f_2 = 4 = a_1(-1)^2 + a_2(1 + \sqrt{3})^2 + a_3(1 - \sqrt{3})^2 \implies a_1 + a_2(4 + 2\sqrt{3}) + a_3(4 - 2\sqrt{3}) = 4$$

$$\implies a_1 + 4a_2 + 2\sqrt{3}a_2 + 4a_3 - 2\sqrt{3}a_3 = 4$$

After solving these systems of equations, we find that:

$$a_1 = 2, a_2 = \frac{5 - 6\sqrt{3}}{2\sqrt{3}} + 2, a_3 = \frac{5\sqrt{3} - 6}{6}$$

The final solution is: $2(-1)^n + (\frac{5 - 6\sqrt{3}}{2\sqrt{3}} + 2)(1 + \sqrt{3})^n + (\frac{5\sqrt{3} - 6}{6})(1 - \sqrt{3})^n$.

b)

$$t_n = t_{n-1} + 2t_{n-2} + 2^n$$

$$t_0 = 0$$

$$t_1 = 2$$

Show your work (all steps: the associated homogeneous equation, the characteristic polynomial and its roots, the general solution of the homogeneous equation, computing a particular solution, the general solution of the non-homogeneous equation, using the initial conditions to compute the final solution.)

Solution:

Characteristic polynomial and its roots: $x^2 - x - 2 = 0, x_1 = -1, x_2 = 2$

General solution of the homogeneous equation: $f'_n = a_1(-1)^n + a_2(2)^n, q(n) = 2^n$.

A particular solution of the form: $f''_n = \beta n 2^n$,

$$\beta n 2^n = \beta(n-1)2^{n-1} + 2\beta(n-2)2^{n-2} + 2^n$$

$$n = 2, 8\beta = 2\beta + 0 + 4 \implies 6\beta = 4 \implies \beta = \frac{2}{3}$$

The general form: $t_n = a_1(-1)^n + a_2(2)^n + \frac{2}{3}n2^n$

Using the initial conditions:

$$f_0 = a_1(-1)^0 + a_2(2)^0 + \frac{2}{3} * 0 * 2^0 \implies a_1 + a_2 = 0$$

$$f_1 = a_1(-1)^1 + a_2(2)^1 + \frac{2}{3} * 1 * 2^1 \implies -a_1 + 2a_2 = 2$$

$$a_1 = -\frac{2}{9}, a_2 = \frac{2}{9}$$

The final solution: $t_n = -\frac{2}{9}(-1)^n + \frac{2}{9}(2)^n + \frac{2}{3}n2^n$

Problem 3: We want to tile an $n \times 1$ strip with 1×1 tiles that are green (G), blue (B), and red (R), 2×1 purple (P) and 2×1 orange (O) tiles. Green, blue and purple tiles cannot be next to each other, and there should be no two purple or three blue or green tiles in a row (for ex., GGOBR is allowed, but GGGOBR, GROPP and PBOBR are not). Give a formula for the number of such tilings. Your solution must include a recurrence equation (with initial conditions!), and a full justification. You do not need to solve it.

Solution:

$$t_n = 3t_{n-1} + 2t_{n-2}$$

$$t_0 = 1$$

$$t_1 = 3$$

For $n = 0$, $t_0 = 1$ because this is just one tiling that has no tiles. For $n = 1$, $t_1 = 3$ because we have three 1×1 tiles. Together, we get the above as the recurrence equation because we have two different types of

tilings: 1×1 tiles and 2×1 tiles. We have three 1×1 tiles, representing $3t_{n-1}$, and two 2×1 tiles, representing $2t_{n-2}$. By adding those two expressions, we will get the number of tilings.

Academic integrity declaration. We, Hugo Wan and Binh Le, did the assignment together.